some proofs #116

untimed/NewSpfStep.thy
@@ -12,10 +12,27 @@ typedef 'm sbElem = "{x :: (channel\<rightharpoonup>'m::message) . sbElemWell x}
    by(simp add: sbElemWellEx)
   
 definition sbHdElemWell::"'m::message SB \<Rightarrow> bool" where
-"sbHdElemWell sb = (\<forall>c \<in> ubDom\<cdot>(sb). sb. c \<noteq> \<epsilon>)"  
+"sbHdElemWell  \<equiv> \<lambda> sb. (\<forall>c \<in> ubDom\<cdot>(sb). sb. c \<noteq> \<epsilon>)"  
+
+lemma sbHdElemWell_mono[simp]:"monofun (\<lambda> sb. (\<forall>c \<in> ubDom\<cdot>(sb). sb. c \<noteq> \<epsilon>))"
+  apply(rule monofunI, simp add: less_bool_def)
+  by (metis bottomI ubdom_below ubgetch_below)
+(*    
+lemma "cont (\<lambda> sb. (\<forall>c \<in> ubDom\<cdot>(sb). sb. c \<noteq> \<epsilon>))"
+proof(rule Cont.contI2, simp)
+  fix Y::"nat \<Rightarrow> 'a stream\<^sup>\<Omega>"
+  assume a1:"chain Y"
+  assume a2:"chain (\<lambda>i::nat. \<forall>c::channel\<in>ubDom\<cdot>(Y i). Y i  .  c \<noteq> \<epsilon>)"
+  show "(\<forall>c::channel\<in>ubDom\<cdot>(\<Squnion>i::nat. Y i). (\<Squnion>i::nat. Y i)  .  c \<noteq> \<epsilon>) \<sqsubseteq> (\<Squnion>i::nat. \<forall>c::channel\<in>ubDom\<cdot>(Y i). Y i  .  c \<noteq> \<epsilon>)"
+    apply(simp add: less_bool_def)
+    apply(subst contlub_cfun_arg, simp add: a1)
+    sorry
+qed
+  *)
+    
 
 lemma sbHdElemWell_inv_ex:"sbHdElemWell sb \<Longrightarrow> \<exists>x. convDiscrUp x = (sbHdElem\<cdot>sb)"
-  using convdiscrup_inv_eq sbHdElemWell_def sbHdElem_dom sbHdElem_channel by blast
+  by (metis convdiscrup_inv_eq sbHdElemWell_def sbHdElem_channel sbHdElem_dom)
 
 lemma sbHdElemWell_invConvDiscrUp:"sbHdElemWell sb \<Longrightarrow> \<forall>c\<in>ubDom\<cdot>(sb).((inv convDiscrUp) (sbHdElem\<cdot>sb)) \<rightharpoonup> c = inv Discr (inv Iup ((sbHdElem\<cdot>sb) \<rightharpoonup> c))"
   by (simp add: convDiscrUp_inv_subst sbHdElemWell_def sbHdElem_channel)
@@ -32,31 +49,178 @@ proof
     using a1 a2 a3 lshd_eq ubgetch_below by blast
 qed
   
-     
+  
 (* updis bijectiv *)
 thm inv_def
 (* Returns the SPF that switches depending on input.  (spfStep_h1 In Out\<cdot>h)\<cdot>(sbHdElem\<cdot>sb) computes the SPF which has to be applied to the input sb*)
-definition spfStep_inj :: "channel set \<Rightarrow> channel set \<Rightarrow> ('m::message sbElem \<Rightarrow> 'm SPF) \<rightarrow> ( 'm SB \<rightarrow>'m SPF)" where
+definition spfStep_inj :: "channel set \<Rightarrow> channel set \<Rightarrow> ('m::message sbElem \<Rightarrow> 'm SPF) \<rightarrow> 'm SB \<rightarrow>'m SPF" where
 "spfStep_inj In Out \<equiv> (\<Lambda> h. (\<Lambda> sb. (if (sbHdElemWell sb) then ufRestrict In Out\<cdot>(h (Abs_sbElem(inv convDiscrUp (sbHdElem\<cdot>sb)))) else ufLeast In Out)))"
 
-
+(*
 definition spfStep_apply::"channel set \<Rightarrow> channel set \<Rightarrow> ('m::message sbElem \<Rightarrow> 'm SPF) \<rightarrow> 'm SB \<rightarrow> 'm SPF"where
-"spfStep_apply In Out \<equiv> \<Lambda> h. (\<Lambda> sb1. Abs_ufun(\<Lambda> sb2. (ubDom\<cdot>sb2 = In) \<leadsto> ((spfStep_inj In Out\<cdot>h)\<cdot>sb1) \<rightleftharpoons> sb2 ))"
+"spfStep_apply In Out \<equiv> \<Lambda> h. (\<Lambda> sb1. (spfStep_inj In Out\<cdot>h)\<cdot>sb1)"
+*)
+
+(*inj_on test*)
+
+lemma spfStep_inj_mono_h[simp]:"monofun (\<lambda> sb. (if (sbHdElemWell sb) then ufRestrict In Out\<cdot>(h (Abs_sbElem(inv convDiscrUp (sbHdElem\<cdot>sb)))) else ufLeast In Out))"
+proof(rule monofunI)
+  fix x y::"'a stream\<^sup>\<Omega>"
+  assume a1:"x \<sqsubseteq> y"
+  show "(if sbHdElemWell x then ufRestrict In Out\<cdot>(h (Abs_sbElem (inv convDiscrUp (sbHdElem\<cdot>x)))) else ufLeast In Out) \<sqsubseteq>
+       (if sbHdElemWell y then ufRestrict In Out\<cdot>(h (Abs_sbElem (inv convDiscrUp (sbHdElem\<cdot>y)))) else ufLeast In Out)"
+  proof(cases "sbHdElemWell x")
+    case True
+    then have true_y:"sbHdElemWell y"
+      by (metis a1 bottomI sbHdElemWell_def ubdom_below ubgetch_below)
+    have a3:"sbHdElem\<cdot>x = sbHdElem\<cdot>y"
+        apply(rule sbHdElem_eq)
+        apply (meson True sbHdElemWell_def)
+        using True sbHdElemWell_def a1 by blast
+    have "ufRestrict In Out\<cdot>(h (Abs_sbElem (inv convDiscrUp (sbHdElem\<cdot>x)))) \<sqsubseteq> ufRestrict In Out\<cdot>(h (Abs_sbElem (inv convDiscrUp (sbHdElem\<cdot>y))))"
+        by (smt a1 a3 below_option_def po_eq_conv spfrt_step ufun_rel_eq)
+    then show ?thesis
+      by(simp add: True true_y)  
+  next
+    case False
+    then show ?thesis
+      by auto
+  qed
+qed
+  
+
+lemma spfStep_inj_cont_h[simp]:"cont (\<lambda> sb. (if (sbHdElemWell sb) then ufRestrict In Out\<cdot>(h (Abs_sbElem(inv convDiscrUp (sbHdElem\<cdot>sb)))) else ufLeast In Out))"(*Maybe In has to be finite for cont*)
+proof(rule Cont.contI2, simp)
+  fix Y::"nat \<Rightarrow> 'a stream\<^sup>\<Omega>"
+  assume a1:"chain Y"
+  assume a2:"chain (\<lambda>i. if sbHdElemWell (Y i) then ufRestrict In Out\<cdot>(h (Abs_sbElem (inv convDiscrUp (sbHdElem\<cdot>(Y i))))) else ufLeast In Out)"
+  show "(if sbHdElemWell (\<Squnion>i. Y i) then ufRestrict In Out\<cdot>(h (Abs_sbElem (inv convDiscrUp (sbHdElem\<cdot>(\<Squnion>i. Y i))))) else ufLeast In Out) \<sqsubseteq>
+       (\<Squnion>i. if sbHdElemWell (Y i) then ufRestrict In Out\<cdot>(h (Abs_sbElem (inv convDiscrUp (sbHdElem\<cdot>(Y i))))) else ufLeast In Out)"
+  proof(cases "sbHdElemWell (\<Squnion>i. Y i)")
+    case True
+    then show ?thesis sorry
+  next
+    case False
+    then show ?thesis sorry
+  qed
+qed
+  
+lemma spfStep_inj_mono[simp]:"monofun (\<lambda> h. (\<Lambda> sb. (if (sbHdElemWell sb) then ufRestrict In Out\<cdot>(h (Abs_sbElem(inv convDiscrUp (sbHdElem\<cdot>sb)))) else ufLeast In Out)))"
+proof(rule monofunI)
+  fix x y ::"'a sbElem \<Rightarrow> 'b ufun"
+  assume a1:"x \<sqsubseteq> y"
+  show "(\<Lambda> sb. if sbHdElemWell sb then ufRestrict In Out\<cdot>(x (Abs_sbElem (inv convDiscrUp (sbHdElem\<cdot>sb)))) else ufLeast In Out) \<sqsubseteq>
+       (\<Lambda> sb. if sbHdElemWell sb then ufRestrict In Out\<cdot>(y (Abs_sbElem (inv convDiscrUp (sbHdElem\<cdot>sb)))) else ufLeast In Out)"
+  proof(rule cfun_belowI,auto)
+    fix xa::"'a stream\<^sup>\<Omega>"
+    assume a2:"sbHdElemWell xa"
+    show "ufRestrict In Out\<cdot>(x (Abs_sbElem (inv convDiscrUp (sbHdElem\<cdot>xa)))) \<sqsubseteq> ufRestrict In Out\<cdot>(y (Abs_sbElem (inv convDiscrUp (sbHdElem\<cdot>xa))))"
+      by (simp add: a1 cont_pref_eq1I fun_belowD)
+  qed
+qed
+    
+
+lemma spfStep_inj_cont[simp]:"cont (\<lambda> h. (\<Lambda> sb. (if (sbHdElemWell sb) then ufRestrict In Out\<cdot>(h (Abs_sbElem(inv convDiscrUp (sbHdElem\<cdot>sb)))) else ufLeast In Out)))"
+proof(rule Cont.contI2, simp)
+  fix Y::"nat \<Rightarrow> 'a sbElem \<Rightarrow> 'b ufun"
+  assume a1: "chain Y"
+  assume a2: "chain (\<lambda>i::nat. \<Lambda> (sb::'a stream\<^sup>\<Omega>). if sbHdElemWell sb then ufRestrict In Out\<cdot>(Y i (Abs_sbElem (inv convDiscrUp (sbHdElem\<cdot>sb)))) else ufLeast In Out)"
+  show "(\<Lambda> sb. if sbHdElemWell sb then ufRestrict In Out\<cdot>((\<Squnion>i::nat. Y i) (Abs_sbElem (inv convDiscrUp (sbHdElem\<cdot>sb)))) else ufLeast In Out) \<sqsubseteq>
+       (\<Squnion>i. \<Lambda> sb. if sbHdElemWell sb then ufRestrict In Out\<cdot>(Y i (Abs_sbElem (inv convDiscrUp (sbHdElem\<cdot>sb)))) else ufLeast In Out)"
+    sorry
+qed
+  
+        
+    
+lemma sbElem_surj_h:" \<exists>sb. f = (inv convDiscrUp (sbHdElem\<cdot>sb)) \<and> sbHdElemWell sb"
+proof-    
+  show "\<exists>sb. f = inv convDiscrUp (sbHdElem\<cdot>sb) \<and> sbHdElemWell sb"
+    sorry
+qed
+          
+lemma sbElem_surj:"\<exists>sb. sbE =  Abs_sbElem (inv convDiscrUp (sbHdElem\<cdot>sb)) \<and> sbHdElemWell sb"
+  sorry
+    
+lemma spfStep_inj_on:"inj_on (Rep_cfun (spfStep_inj In Out)) {h. \<forall>m. ufDom\<cdot>(h m) = In \<and> ufRan\<cdot>(h m) = Out}"
+proof(simp add: spfStep_inj_def, rule inj_onI)
+  fix x y :: "'a sbElem \<Rightarrow> ('a stream\<^sup>\<Omega>) ufun"
+  assume ax:" x \<in> {h. \<forall>m. ufDom\<cdot>(h m) = In \<and> ufRan\<cdot>(h m) = Out}"
+  assume ay:" y \<in> {h. \<forall>m. ufDom\<cdot>(h m) = In \<and> ufRan\<cdot>(h m) = Out}"
+  assume a1:"(\<Lambda> sb. if sbHdElemWell sb then ufRestrict In Out\<cdot>(x (Abs_sbElem (inv convDiscrUp (sbHdElem\<cdot>sb)))) else ufLeast In Out) =
+             (\<Lambda> sb. if sbHdElemWell sb then ufRestrict In Out\<cdot>(y (Abs_sbElem (inv convDiscrUp (sbHdElem\<cdot>sb)))) else ufLeast In Out)"
+  have ya:"(\<forall>elem.  ufDom\<cdot>(y elem) = In \<and> ufRan\<cdot>(y elem) = Out)"
+    using ay by auto
+  have xa:"(\<forall>elem.  ufDom\<cdot>(x elem) = In \<and> ufRan\<cdot>(x elem) = Out)"
+    using ax by auto
+  show "x = y"
+  proof(cases "x \<noteq> y")
+    case True
+    then obtain sbE where sbE_def:" x sbE \<noteq> y sbE"
+      by fastforce
+    then obtain sb where sb_def:"((inv convDiscrUp (sbHdElem\<cdot>sb))) =  (Rep_sbElem sbE) \<and> sbHdElemWell sb"
+      using sbElem_surj_h  by metis
+    then have spf_uneq:"(x (Abs_sbElem (inv convDiscrUp (sbHdElem\<cdot>sb)))) \<noteq> (y (Abs_sbElem (inv convDiscrUp (sbHdElem\<cdot>sb))))"
+      by(simp add: Rep_sbElem_inverse sb_def sbE_def)
+    obtain spf1 where spf_1_def:" (x (Abs_sbElem (inv convDiscrUp (sbHdElem\<cdot>sb)))) = spf1"
+      by simp
+    obtain spf2 where spf_2_def:" (y (Abs_sbElem (inv convDiscrUp (sbHdElem\<cdot>sb)))) = spf2"
+      by simp
+    have ufR_uneq:"ufRestrict In Out\<cdot>spf1 \<noteq> ufRestrict In Out\<cdot>spf2"
+      using ax ya spf_uneq spf_1_def spf_2_def by auto
+    have uf_eq:"ufRestrict In Out\<cdot>spf1 = spf1 \<and> ufRestrict In Out\<cdot>spf2 = spf2"
+      using ax spf_1_def spf_2_def ya by auto
+    then have "spf1 \<noteq> spf2"
+      using ufR_uneq by auto
+    have sb_Well:"sbHdElemWell sb"
+      by(simp add: sb_def)
+    have h:"(\<lambda> sb. if sbHdElemWell sb then ufRestrict In Out\<cdot>(x (Abs_sbElem (inv convDiscrUp (sbHdElem\<cdot>sb)))) else ufLeast In Out) \<noteq>
+             (\<lambda> sb. if sbHdElemWell sb then ufRestrict In Out\<cdot>(y (Abs_sbElem (inv convDiscrUp (sbHdElem\<cdot>sb)))) else ufLeast In Out)"
+      apply(subst fun_eq_iff,auto)
+      apply(rule_tac x="sb" in exI)
+      by(simp add: spf_1_def spf_2_def ufR_uneq sb_Well)
+    have "(\<Lambda> sb. if sbHdElemWell sb then ufRestrict In Out\<cdot>(x (Abs_sbElem (inv convDiscrUp (sbHdElem\<cdot>sb)))) else ufLeast In Out) \<noteq>
+             (\<Lambda> sb. if sbHdElemWell sb then ufRestrict In Out\<cdot>(y (Abs_sbElem (inv convDiscrUp (sbHdElem\<cdot>sb)))) else ufLeast In Out)"
+      apply(subst cfun_eq_iff, auto)
+      apply(rule_tac x="sb" in exI)
+      by(simp add: spf_1_def spf_2_def ufR_uneq sb_Well)
+    then show ?thesis
+      by(simp add: a1)
+  next
+    case False
+    then show ?thesis 
+      by simp
+  qed
+qed
+  
+
+
+
+
+
+
+
+
+
+
+
+
+
+(*other definition*)
 
 definition spfStep ::"channel set \<Rightarrow> channel set \<Rightarrow> ('m::message sbElem \<Rightarrow> 'm SPF) \<rightarrow> 'm SPF" where
 "spfStep In Out \<equiv> \<Lambda> h. Abs_ufun (\<Lambda>  sb.  (ubDom\<cdot>sb = In) 
-                                              \<leadsto> (if (sbHdElemWell sb) then ufRestrict In Out\<cdot>(h (Abs_sbElem(inv convDiscrUp (sbHdElem\<cdot>sb)))) \<rightleftharpoons> (sbRt\<cdot>sb) else ubclLeast Out))"
+                                              \<leadsto> (if (sbHdElemWell sb) then ufRestrict In Out\<cdot>(h (Abs_sbElem(inv convDiscrUp (sbHdElem\<cdot>sb)))) \<rightleftharpoons> sb else ubclLeast Out))"
 
 
 lemma spfStep_innerMono:"monofun (\<lambda>  sb.  (ubDom\<cdot>sb = In) 
-                                              \<leadsto> (if (sbHdElemWell sb) then ufRestrict In Out\<cdot>(h (Abs_sbElem(inv convDiscrUp (sbHdElem\<cdot>sb)))) \<rightleftharpoons> (sbRt\<cdot>sb) else ubclLeast Out))"
+                                              \<leadsto> (if (sbHdElemWell sb) then ufRestrict In Out\<cdot>(h (Abs_sbElem(inv convDiscrUp (sbHdElem\<cdot>sb)))) \<rightleftharpoons> sb else ubclLeast Out))"
 proof(rule monofunI)
   fix x y::"'a stream\<^sup>\<Omega>"
   assume a1:"x\<sqsubseteq>y"
   have a2:"(ubDom\<cdot>x = In \<and> sbHdElemWell x) \<Longrightarrow> (ubDom\<cdot>y = In \<and> sbHdElemWell y)"
     by (metis a1 below_bottom_iff sbHdElemWell_def ubdom_below ubgetch_below)
-  show "(ubDom\<cdot>x = In)\<leadsto>if sbHdElemWell x then ufRestrict In Out\<cdot>(h (Abs_sbElem (inv convDiscrUp (sbHdElem\<cdot>x)))) \<rightleftharpoons> sbRt\<cdot>x else ubclLeast Out \<sqsubseteq>
-       (ubDom\<cdot>y = In)\<leadsto>if sbHdElemWell y then ufRestrict In Out\<cdot>(h (Abs_sbElem (inv convDiscrUp (sbHdElem\<cdot>y)))) \<rightleftharpoons> sbRt\<cdot>y else ubclLeast Out"
+  show "(ubDom\<cdot>x = In)\<leadsto>if sbHdElemWell x then ufRestrict In Out\<cdot>(h (Abs_sbElem (inv convDiscrUp (sbHdElem\<cdot>x)))) \<rightleftharpoons> x else ubclLeast Out \<sqsubseteq>
+       (ubDom\<cdot>y = In)\<leadsto>if sbHdElemWell y then ufRestrict In Out\<cdot>(h (Abs_sbElem (inv convDiscrUp (sbHdElem\<cdot>y)))) \<rightleftharpoons>y else ubclLeast Out"
   proof(cases "ubDom\<cdot>x = In")
     case True
     then have true_x:"ubDom\<cdot>x = In"
@@ -70,8 +234,9 @@ proof(rule monofunI)
         using True a1 a2 true_y ubdom_below by auto
       have a3:"sbHdElem\<cdot>x = sbHdElem\<cdot>y"
         apply(rule sbHdElem_eq)
-        using True sbHdElemWell_def a1 by blast+
-      have "(ufRestrict In Out\<cdot>(h (Abs_sbElem (inv convDiscrUp (sbHdElem\<cdot>x)))) \<rightleftharpoons> sbRt\<cdot>x) \<sqsubseteq> (ufRestrict In Out\<cdot>(h (Abs_sbElem (inv convDiscrUp (sbHdElem\<cdot>y)))) \<rightleftharpoons> sbRt\<cdot>y)"
+        apply (meson True sbHdElemWell_def)
+        using True sbHdElemWell_def a1 by blast
+      have "(ufRestrict In Out\<cdot>(h (Abs_sbElem (inv convDiscrUp (sbHdElem\<cdot>x)))) \<rightleftharpoons> x) \<sqsubseteq> (ufRestrict In Out\<cdot>(h (Abs_sbElem (inv convDiscrUp (sbHdElem\<cdot>y)))) \<rightleftharpoons> y)"
         by (smt a1 a3 below_option_def po_eq_conv spfrt_step ufun_rel_eq)
       then show ?thesis
         by(simp add: True true_x true_y true_y2 some_below)
@@ -89,67 +254,82 @@ qed
   
 
 lemma spfStep_innerCont:"cont (\<lambda>  sb.  (ubDom\<cdot>sb = In) 
-                                              \<leadsto> (if (sbHdElemWell sb) then ufRestrict In Out\<cdot>(h (Abs_sbElem(inv convDiscrUp (sbHdElem\<cdot>sb)))) \<rightleftharpoons> (sbRt\<cdot>sb) else ubclLeast Out))"
+                                              \<leadsto> (if (sbHdElemWell sb) then ufRestrict In Out\<cdot>(h (Abs_sbElem(inv convDiscrUp (sbHdElem\<cdot>sb)))) \<rightleftharpoons> sb else ubclLeast Out))"
 proof(rule Cont.contI2, simp add: spfStep_innerMono)
   fix Y::"nat \<Rightarrow> 'a stream\<^sup>\<Omega>"
   assume a1:"chain Y"
-  assume a2:"chain (\<lambda>i::nat. (ubDom\<cdot>(Y i) = In)\<leadsto>if sbHdElemWell (Y i) then ufRestrict In Out\<cdot>(h (Abs_sbElem (inv convDiscrUp (sbHdElem\<cdot>(Y i))))) \<rightleftharpoons> sbRt\<cdot>(Y i) else ubclLeast Out)"
+  assume a2:"chain (\<lambda>i::nat. (ubDom\<cdot>(Y i) = In)\<leadsto>if sbHdElemWell (Y i) then ufRestrict In Out\<cdot>(h (Abs_sbElem (inv convDiscrUp (sbHdElem\<cdot>(Y i))))) \<rightleftharpoons> (Y i) else ubclLeast Out)"
   show "(ubDom\<cdot>(\<Squnion>i. Y i) = In)\<leadsto>if sbHdElemWell (\<Squnion>i. Y i) then 
-        ufRestrict In Out\<cdot>(h (Abs_sbElem (inv convDiscrUp (sbHdElem\<cdot>(\<Squnion>i. Y i))))) \<rightleftharpoons> sbRt\<cdot>(\<Squnion>i. Y i) else ubclLeast Out \<sqsubseteq>
+        ufRestrict In Out\<cdot>(h (Abs_sbElem (inv convDiscrUp (sbHdElem\<cdot>(\<Squnion>i. Y i))))) \<rightleftharpoons> (\<Squnion>i. Y i) else ubclLeast Out \<sqsubseteq>
         (\<Squnion>i. (ubDom\<cdot>(Y i) = In)\<leadsto>if sbHdElemWell (Y i) then 
-        ufRestrict In Out\<cdot>(h (Abs_sbElem (inv convDiscrUp (sbHdElem\<cdot>(Y i))))) \<rightleftharpoons> sbRt\<cdot>(Y i) else ubclLeast Out)"
+        ufRestrict In Out\<cdot>(h (Abs_sbElem (inv convDiscrUp (sbHdElem\<cdot>(Y i))))) \<rightleftharpoons>(Y i) else ubclLeast Out)"
     sorry
 qed
   
 
 lemma spfStep_innerWell:"ufWell (\<Lambda>  sb.  (ubDom\<cdot>sb = In) 
-                                              \<leadsto> (if (sbHdElemWell sb) then ufRestrict In Out\<cdot>(h (Abs_sbElem(inv convDiscrUp (sbHdElem\<cdot>sb)))) \<rightleftharpoons> (sbRt\<cdot>sb) else ubclLeast Out)) "
+                                              \<leadsto> (if (sbHdElemWell sb) then ufRestrict In Out\<cdot>(h (Abs_sbElem(inv convDiscrUp (sbHdElem\<cdot>sb)))) \<rightleftharpoons> sb else ubclLeast Out)) "
 proof(simp add: ufWell_def)
   fix b::"'a stream\<^sup>\<Omega>"
   have In:"\<forall>b.(b \<in> dom (Rep_cfun (\<Lambda> (sb::'a stream\<^sup>\<Omega>).
-                                   (ubDom\<cdot>sb = In)\<leadsto>if sbHdElemWell sb then ufRestrict In Out\<cdot>(h (Abs_sbElem (inv convDiscrUp (sbHdElem\<cdot>sb)))) \<rightleftharpoons> sbRt\<cdot>sb else ubclLeast Out))) =
+                                   (ubDom\<cdot>sb = In)\<leadsto>if sbHdElemWell sb then ufRestrict In Out\<cdot>(h (Abs_sbElem (inv convDiscrUp (sbHdElem\<cdot>sb)))) \<rightleftharpoons> sb else ubclLeast Out))) =
            (ubclDom\<cdot>b = In)"
     by (simp add: domIff2 spfStep_innerCont ubclDom_ubundle_def)    
   have Out:"\<forall>b. b \<in> ran (Rep_cfun (\<Lambda> (sb::'a stream\<^sup>\<Omega>).
-                                  (ubDom\<cdot>sb = In)\<leadsto>if sbHdElemWell sb then ufRestrict In Out\<cdot>(h (Abs_sbElem (inv convDiscrUp (sbHdElem\<cdot>sb)))) \<rightleftharpoons> sbRt\<cdot>sb else ubclLeast Out)) \<longrightarrow>
+                                  (ubDom\<cdot>sb = In)\<leadsto>if sbHdElemWell sb then ufRestrict In Out\<cdot>(h (Abs_sbElem (inv convDiscrUp (sbHdElem\<cdot>sb)))) \<rightleftharpoons> sb else ubclLeast Out)) \<longrightarrow>
            ubclDom\<cdot>b = Out"
   sorry
   show "(\<exists>Ina::channel set.
         \<forall>b::'a stream\<^sup>\<Omega>.
            (b \<in> dom (Rep_cfun (\<Lambda> (sb::'a stream\<^sup>\<Omega>).
-                                   (ubDom\<cdot>sb = In)\<leadsto>if sbHdElemWell sb then ufRestrict In Out\<cdot>(h (Abs_sbElem (inv convDiscrUp (sbHdElem\<cdot>sb)))) \<rightleftharpoons> sbRt\<cdot>sb else ubclLeast Out))) =
+                                   (ubDom\<cdot>sb = In)\<leadsto>if sbHdElemWell sb then ufRestrict In Out\<cdot>(h (Abs_sbElem (inv convDiscrUp (sbHdElem\<cdot>sb)))) \<rightleftharpoons> sb else ubclLeast Out))) =
            (ubclDom\<cdot>b = Ina)) \<and>
     (\<exists>Outa::channel set.
         \<forall>b::'a stream\<^sup>\<Omega>.
            b \<in> ran (Rep_cfun (\<Lambda> (sb::'a stream\<^sup>\<Omega>).
-                                  (ubDom\<cdot>sb = In)\<leadsto>if sbHdElemWell sb then ufRestrict In Out\<cdot>(h (Abs_sbElem (inv convDiscrUp (sbHdElem\<cdot>sb)))) \<rightleftharpoons> sbRt\<cdot>sb else ubclLeast Out)) \<longrightarrow>
+                                  (ubDom\<cdot>sb = In)\<leadsto>if sbHdElemWell sb then ufRestrict In Out\<cdot>(h (Abs_sbElem (inv convDiscrUp (sbHdElem\<cdot>sb)))) \<rightleftharpoons> sb else ubclLeast Out)) \<longrightarrow>
            ubclDom\<cdot>b = Outa)"
     using In Out by blast
 qed
   
 lemma spfStep_mono:"monofun (\<lambda> h. Abs_ufun (\<Lambda>  sb.  (ubDom\<cdot>sb = In) 
-                                              \<leadsto> (if (sbHdElemWell sb) then ufRestrict In Out\<cdot>(h (Abs_sbElem(inv convDiscrUp (sbHdElem\<cdot>sb)))) \<rightleftharpoons> (sbRt\<cdot>sb) else ubclLeast Out)))"
+                                              \<leadsto> (if (sbHdElemWell sb) then ufRestrict In Out\<cdot>(h (Abs_sbElem(inv convDiscrUp (sbHdElem\<cdot>sb)))) \<rightleftharpoons> sb else ubclLeast Out)))"
 proof(rule monofunI)
   fix x y ::"'a sbElem \<Rightarrow> ('a stream\<^sup>\<Omega>) ufun"
   assume a1:"x\<sqsubseteq>y"
-  show "Abs_cufun (\<lambda>sb. (ubDom\<cdot>sb = In)\<leadsto>if sbHdElemWell sb then ufRestrict In Out\<cdot>(x (Abs_sbElem (inv convDiscrUp (sbHdElem\<cdot>sb)))) \<rightleftharpoons> sbRt\<cdot>sb else ubclLeast Out) \<sqsubseteq>
-        Abs_cufun (\<lambda>sb. (ubDom\<cdot>sb = In)\<leadsto>if sbHdElemWell sb then ufRestrict In Out\<cdot>(y (Abs_sbElem (inv convDiscrUp (sbHdElem\<cdot>sb)))) \<rightleftharpoons> sbRt\<cdot>sb else ubclLeast Out)"
+  show "Abs_cufun (\<lambda>sb. (ubDom\<cdot>sb = In)\<leadsto>if sbHdElemWell sb then ufRestrict In Out\<cdot>(x (Abs_sbElem (inv convDiscrUp (sbHdElem\<cdot>sb)))) \<rightleftharpoons> sb else ubclLeast Out) \<sqsubseteq>
+        Abs_cufun (\<lambda>sb. (ubDom\<cdot>sb = In)\<leadsto>if sbHdElemWell sb then ufRestrict In Out\<cdot>(y (Abs_sbElem (inv convDiscrUp (sbHdElem\<cdot>sb)))) \<rightleftharpoons> sb else ubclLeast Out)"
   proof(rule ufun_belowI)
     show"ufDom\<cdot>(Abs_cufun (\<lambda>sb::'a stream\<^sup>\<Omega>.
-                         (ubDom\<cdot>sb = In)\<leadsto>if sbHdElemWell sb then ufRestrict In Out\<cdot>(x (Abs_sbElem (inv convDiscrUp (sbHdElem\<cdot>sb)))) \<rightleftharpoons> sbRt\<cdot>sb else ubclLeast Out)) =
-    ufDom\<cdot>(Abs_cufun (\<lambda>sb::'a stream\<^sup>\<Omega>. (ubDom\<cdot>sb = In)\<leadsto>if sbHdElemWell sb then ufRestrict In Out\<cdot>(y (Abs_sbElem (inv convDiscrUp (sbHdElem\<cdot>sb)))) \<rightleftharpoons> sbRt\<cdot>sb else ubclLeast Out))"
+                         (ubDom\<cdot>sb = In)\<leadsto>if sbHdElemWell sb then ufRestrict In Out\<cdot>(x (Abs_sbElem (inv convDiscrUp (sbHdElem\<cdot>sb)))) \<rightleftharpoons> sb else ubclLeast Out)) =
+    ufDom\<cdot>(Abs_cufun (\<lambda>sb::'a stream\<^sup>\<Omega>. (ubDom\<cdot>sb = In)\<leadsto>if sbHdElemWell sb then ufRestrict In Out\<cdot>(y (Abs_sbElem (inv convDiscrUp (sbHdElem\<cdot>sb)))) \<rightleftharpoons> sb else ubclLeast Out))"
       apply(simp add: spfStep_innerCont spfStep_innerWell ufdom_insert )
+      sorry
+  next
+    show "\<And>xa::'a stream\<^sup>\<Omega>.
+       ubclDom\<cdot>xa =
+       ufDom\<cdot>(Abs_cufun (\<lambda>sb::'a stream\<^sup>\<Omega>.
+                            (ubDom\<cdot>sb = In)\<leadsto>if sbHdElemWell sb then ufRestrict In Out\<cdot>(x (Abs_sbElem (inv convDiscrUp (sbHdElem\<cdot>sb)))) \<rightleftharpoons> sb else ubclLeast Out)) \<Longrightarrow>
+       Abs_cufun (\<lambda>sb::'a stream\<^sup>\<Omega>. (ubDom\<cdot>sb = In)\<leadsto>if sbHdElemWell sb then ufRestrict In Out\<cdot>(x (Abs_sbElem (inv convDiscrUp (sbHdElem\<cdot>sb)))) \<rightleftharpoons> sb else ubclLeast Out) \<rightleftharpoons> xa \<sqsubseteq>
+       Abs_cufun (\<lambda>sb::'a stream\<^sup>\<Omega>. (ubDom\<cdot>sb = In)\<leadsto>if sbHdElemWell sb then ufRestrict In Out\<cdot>(y (Abs_sbElem (inv convDiscrUp (sbHdElem\<cdot>sb)))) \<rightleftharpoons> sb else ubclLeast Out) \<rightleftharpoons> xa"
+      sorry
+  qed
+qed
+  
+    
+
+(*
     proof -
       { fix uu :: "'a stream\<^sup>\<Omega>"
-        have "ubDom\<cdot>uu = In \<longrightarrow> uu \<notin> dom (\<lambda>u. (ubDom\<cdot>u = In)\<leadsto>if sbHdElemWell u then ufRestrict In Out\<cdot> (y (Abs_sbElem (inv convDiscrUp (sbHdElem\<cdot>u)))) \<rightleftharpoons> sbRt\<cdot>u else ubclLeast Out) \<and> uu \<notin> dom (\<lambda>u. (ubDom\<cdot>u = In)\<leadsto>if sbHdElemWell u then ufRestrict In Out\<cdot> (x (Abs_sbElem (inv convDiscrUp (sbHdElem\<cdot>u)))) \<rightleftharpoons> sbRt\<cdot>u else ubclLeast Out) \<or> uu \<in> dom (\<lambda>u. (ubDom\<cdot>u = In)\<leadsto>if sbHdElemWell u then ufRestrict In Out\<cdot> (x (Abs_sbElem (inv convDiscrUp (sbHdElem\<cdot>u)))) \<rightleftharpoons> sbRt\<cdot>u else ubclLeast Out) \<and> uu \<in> dom (\<lambda>u. (ubDom\<cdot>u = In)\<leadsto>if sbHdElemWell u then ufRestrict In Out\<cdot> (y (Abs_sbElem (inv convDiscrUp (sbHdElem\<cdot>u)))) \<rightleftharpoons> sbRt\<cdot>u else ubclLeast Out)"
+        have "ubDom\<cdot>uu = In \<longrightarrow> uu \<notin> dom (\<lambda>u. (ubDom\<cdot>u = In)\<leadsto>if sbHdElemWell u then ufRestrict In Out\<cdot> (y (Abs_sbElem (inv convDiscrUp (sbHdElem\<cdot>u)))) \<rightleftharpoons> u else ubclLeast Out) \<and> uu \<notin> dom (\<lambda>u. (ubDom\<cdot>u = In)\<leadsto>if sbHdElemWell u then ufRestrict In Out\<cdot> (x (Abs_sbElem (inv convDiscrUp (sbHdElem\<cdot>u)))) \<rightleftharpoons> sbRt\<cdot>u else ubclLeast Out) \<or> uu \<in> dom (\<lambda>u. (ubDom\<cdot>u = In)\<leadsto>if sbHdElemWell u then ufRestrict In Out\<cdot> (x (Abs_sbElem (inv convDiscrUp (sbHdElem\<cdot>u)))) \<rightleftharpoons> sbRt\<cdot>u else ubclLeast Out) \<and> uu \<in> dom (\<lambda>u. (ubDom\<cdot>u = In)\<leadsto>if sbHdElemWell u then ufRestrict In Out\<cdot> (y (Abs_sbElem (inv convDiscrUp (sbHdElem\<cdot>u)))) \<rightleftharpoons> sbRt\<cdot>u else ubclLeast Out)"
           by force
         moreover
         { assume "ubDom\<cdot>uu \<noteq> In"
-          have "uu \<notin> dom (\<lambda>u. (ubDom\<cdot>u = In)\<leadsto>if sbHdElemWell u then ufRestrict In Out\<cdot> (y (Abs_sbElem (inv convDiscrUp (sbHdElem\<cdot>u)))) \<rightleftharpoons> sbRt\<cdot>u else ubclLeast Out) \<and> uu \<notin> dom (\<lambda>u. (ubDom\<cdot>u = In)\<leadsto>if sbHdElemWell u then ufRestrict In Out\<cdot> (x (Abs_sbElem (inv convDiscrUp (sbHdElem\<cdot>u)))) \<rightleftharpoons> sbRt\<cdot>u else ubclLeast Out) \<or> uu \<in> dom (\<lambda>u. (ubDom\<cdot>u = In)\<leadsto>if sbHdElemWell u then ufRestrict In Out\<cdot> (x (Abs_sbElem (inv convDiscrUp (sbHdElem\<cdot>u)))) \<rightleftharpoons> sbRt\<cdot>u else ubclLeast Out) \<and> uu \<in> dom (\<lambda>u. (ubDom\<cdot>u = In)\<leadsto>if sbHdElemWell u then ufRestrict In Out\<cdot> (y (Abs_sbElem (inv convDiscrUp (sbHdElem\<cdot>u)))) \<rightleftharpoons> sbRt\<cdot>u else ubclLeast Out)"
+          have "uu \<notin> dom (\<lambda>u. (ubDom\<cdot>u = In)\<leadsto>if sbHdElemWell u then ufRestrict In Out\<cdot> (y (Abs_sbElem (inv convDiscrUp (sbHdElem\<cdot>u)))) \<rightleftharpoons> u else ubclLeast Out) \<and> uu \<notin> dom (\<lambda>u. (ubDom\<cdot>u = In)\<leadsto>if sbHdElemWell u then ufRestrict In Out\<cdot> (x (Abs_sbElem (inv convDiscrUp (sbHdElem\<cdot>u)))) \<rightleftharpoons> sbRt\<cdot>u else ubclLeast Out) \<or> uu \<in> dom (\<lambda>u. (ubDom\<cdot>u = In)\<leadsto>if sbHdElemWell u then ufRestrict In Out\<cdot> (x (Abs_sbElem (inv convDiscrUp (sbHdElem\<cdot>u)))) \<rightleftharpoons> sbRt\<cdot>u else ubclLeast Out) \<and> uu \<in> dom (\<lambda>u. (ubDom\<cdot>u = In)\<leadsto>if sbHdElemWell u then ufRestrict In Out\<cdot> (y (Abs_sbElem (inv convDiscrUp (sbHdElem\<cdot>u)))) \<rightleftharpoons> sbRt\<cdot>u else ubclLeast Out)"
             by (simp add: dom_def) }
-        ultimately have "uu \<notin> dom (\<lambda>u. (ubDom\<cdot>u = In)\<leadsto>if sbHdElemWell u then ufRestrict In Out\<cdot> (y (Abs_sbElem (inv convDiscrUp (sbHdElem\<cdot>u)))) \<rightleftharpoons> sbRt\<cdot>u else ubclLeast Out) \<and> uu \<notin> dom (\<lambda>u. (ubDom\<cdot>u = In)\<leadsto>if sbHdElemWell u then ufRestrict In Out\<cdot> (x (Abs_sbElem (inv convDiscrUp (sbHdElem\<cdot>u)))) \<rightleftharpoons> sbRt\<cdot>u else ubclLeast Out) \<or> uu \<in> dom (\<lambda>u. (ubDom\<cdot>u = In)\<leadsto>if sbHdElemWell u then ufRestrict In Out\<cdot> (x (Abs_sbElem (inv convDiscrUp (sbHdElem\<cdot>u)))) \<rightleftharpoons> sbRt\<cdot>u else ubclLeast Out) \<and> uu \<in> dom (\<lambda>u. (ubDom\<cdot>u = In)\<leadsto>if sbHdElemWell u then ufRestrict In Out\<cdot> (y (Abs_sbElem (inv convDiscrUp (sbHdElem\<cdot>u)))) \<rightleftharpoons> sbRt\<cdot>u else ubclLeast Out)"
+        ultimately have "uu \<notin> dom (\<lambda>u. (ubDom\<cdot>u = In)\<leadsto>if sbHdElemWell u then ufRestrict In Out\<cdot> (y (Abs_sbElem (inv convDiscrUp (sbHdElem\<cdot>u)))) \<rightleftharpoons> u else ubclLeast Out) \<and> uu \<notin> dom (\<lambda>u. (ubDom\<cdot>u = In)\<leadsto>if sbHdElemWell u then ufRestrict In Out\<cdot> (x (Abs_sbElem (inv convDiscrUp (sbHdElem\<cdot>u)))) \<rightleftharpoons> sbRt\<cdot>u else ubclLeast Out) \<or> uu \<in> dom (\<lambda>u. (ubDom\<cdot>u = In)\<leadsto>if sbHdElemWell u then ufRestrict In Out\<cdot> (x (Abs_sbElem (inv convDiscrUp (sbHdElem\<cdot>u)))) \<rightleftharpoons> sbRt\<cdot>u else ubclLeast Out) \<and> uu \<in> dom (\<lambda>u. (ubDom\<cdot>u = In)\<leadsto>if sbHdElemWell u then ufRestrict In Out\<cdot> (y (Abs_sbElem (inv convDiscrUp (sbHdElem\<cdot>u)))) \<rightleftharpoons> sbRt\<cdot>u else ubclLeast Out)"
           by linarith }
-      then show "ubclDom\<cdot> (SOME u. u \<in> dom (\<lambda>u. (ubDom\<cdot>u = In)\<leadsto>if sbHdElemWell u then ufRestrict In Out\<cdot> (x (Abs_sbElem (inv convDiscrUp (sbHdElem\<cdot>u)))) \<rightleftharpoons> sbRt\<cdot>u else ubclLeast Out)) = ubclDom\<cdot> (SOME u. u \<in> dom (\<lambda>u. (ubDom\<cdot>u = In)\<leadsto>if sbHdElemWell u then ufRestrict In Out\<cdot> (y (Abs_sbElem (inv convDiscrUp (sbHdElem\<cdot>u)))) \<rightleftharpoons> sbRt\<cdot>u else ubclLeast Out))"
+      then show "ubclDom\<cdot> (SOME u. u \<in> dom (\<lambda>u. (ubDom\<cdot>u = In)\<leadsto>if sbHdElemWell u then ufRestrict In Out\<cdot> (x (Abs_sbElem (inv convDiscrUp (sbHdElem\<cdot>u)))) \<rightleftharpoons> u else ubclLeast Out)) = ubclDom\<cdot> (SOME u. u \<in> dom (\<lambda>u. (ubDom\<cdot>u = In)\<leadsto>if sbHdElemWell u then ufRestrict In Out\<cdot> (y (Abs_sbElem (inv convDiscrUp (sbHdElem\<cdot>u)))) \<rightleftharpoons> sbRt\<cdot>u else ubclLeast Out))"
         by meson
     qed
   next
@@ -181,28 +361,61 @@ proof(rule monofunI)
         qed
       qed
   qed   
-qed
+qed*)
   
 
 
 lemma spfStep_cont:"cont (\<lambda> h. Abs_ufun (\<Lambda>  sb.  (ubDom\<cdot>sb = In) 
-                                              \<leadsto> (if (sbHdElemWell sb) then ufRestrict In Out\<cdot>(h (Abs_sbElem(inv convDiscrUp (sbHdElem\<cdot>sb)))) \<rightleftharpoons> (sbRt\<cdot>sb) else ubclLeast Out)))"
-  sorry
-    
-lemma sbElem_surj_h:" \<exists>sb. f = (inv convDiscrUp (sbHdElem\<cdot>sb))"
-proof-
-  obtain sb where sb_def:"\<forall>c\<in>dom f. shd(sb . c) = f \<rightharpoonup> c"
-    sorry
-  then have "f = inv convDiscrUp (sbHdElem\<cdot>sb)"
-      sorry
-  then show "\<exists>sb::'a stream\<^sup>\<Omega>. f = inv convDiscrUp (sbHdElem\<cdot>sb)"
-    by auto
-  qed
-    
-    
-lemma sbElem_surj:"\<exists>sb. sbE=  Abs_sbElem (inv convDiscrUp (sbHdElem\<cdot>sb))"
+                                              \<leadsto> (if (sbHdElemWell sb) then ufRestrict In Out\<cdot>(h (Abs_sbElem(inv convDiscrUp (sbHdElem\<cdot>sb)))) \<rightleftharpoons> sb else ubclLeast Out)))"
   sorry
 
+
+lemma ufDom_uneq:assumes "ubDom\<cdot>sb \<noteq> ufDom\<cdot>spf" shows "spf \<rightleftharpoons> sb = the None"
+  sorry
+    
+    
+lemma "spfStep In Out\<cdot>h \<rightleftharpoons> sb = spfStep_inj In Out\<cdot>h\<cdot>sb \<rightleftharpoons> sb"
+proof(simp add: spfStep_def spfStep_inj_def spfStep_cont, auto)
+  assume a1:"sbHdElemWell sb"
+  show "Abs_cufun (\<lambda>sb::'a stream\<^sup>\<Omega>. (ubDom\<cdot>sb = In)\<leadsto>if sbHdElemWell sb then ufRestrict In Out\<cdot>(h (Abs_sbElem (inv convDiscrUp (sbHdElem\<cdot>sb)))) \<rightleftharpoons> sb else ubclLeast Out) \<rightleftharpoons> sb =
+    ufRestrict In Out\<cdot>(h (Abs_sbElem (inv convDiscrUp (sbHdElem\<cdot>sb)))) \<rightleftharpoons> sb"
+  proof(cases "ubDom\<cdot>sb = In")
+    case True
+    then have h1:"Abs_cufun (\<lambda>sb::'a stream\<^sup>\<Omega>. (ubDom\<cdot>sb = In)\<leadsto>if sbHdElemWell sb then ufRestrict In Out\<cdot>(h (Abs_sbElem (inv convDiscrUp (sbHdElem\<cdot>sb)))) \<rightleftharpoons> sb else ubclLeast Out) \<rightleftharpoons> sb =
+               (if sbHdElemWell sb then ufRestrict In Out\<cdot>(h (Abs_sbElem (inv convDiscrUp (sbHdElem\<cdot>sb)))) \<rightleftharpoons> sb else ubclLeast Out)"
+      sorry
+    show ?thesis
+      by(simp add: h1 True a1)
+  next
+    case False
+    then have h1:"Abs_cufun (\<lambda>sb::'a stream\<^sup>\<Omega>. (ubDom\<cdot>sb = In)\<leadsto>if sbHdElemWell sb then ufRestrict In Out\<cdot>(h (Abs_sbElem (inv convDiscrUp (sbHdElem\<cdot>sb)))) \<rightleftharpoons> sb else ubclLeast Out) \<rightleftharpoons> sb = the None"
+      sorry
+    then show ?thesis
+      by(simp add: ufLeast_def ufDom_uneq False)
+  qed
+next
+  assume a1:"\<not>(sbHdElemWell sb)"
+  show "Abs_cufun (\<lambda>sb::'a stream\<^sup>\<Omega>. (ubDom\<cdot>sb = In)\<leadsto>if sbHdElemWell sb then ufRestrict In Out\<cdot>(h (Abs_sbElem (inv convDiscrUp (sbHdElem\<cdot>sb)))) \<rightleftharpoons> sb else ubclLeast Out) \<rightleftharpoons> sb =
+    ufLeast In Out \<rightleftharpoons> sb"    
+    proof(cases "ubDom\<cdot>sb = In")
+    case True
+    then have h1:"Abs_cufun (\<lambda>sb::'a stream\<^sup>\<Omega>. (ubDom\<cdot>sb = In)\<leadsto>if sbHdElemWell sb then ufRestrict In Out\<cdot>(h (Abs_sbElem (inv convDiscrUp (sbHdElem\<cdot>sb)))) \<rightleftharpoons> sb else ubclLeast Out) \<rightleftharpoons> sb =
+               (if sbHdElemWell sb then ufRestrict In Out\<cdot>(h (Abs_sbElem (inv convDiscrUp (sbHdElem\<cdot>sb)))) \<rightleftharpoons> sb else ubclLeast Out)"
+      sorry
+    show ?thesis
+      apply(simp add: a1 h1 True ufLeast_def)
+      by (simp add: True ubclDom_ubundle_def)
+  next
+    case False
+    then have h1:"Abs_cufun (\<lambda>sb::'a stream\<^sup>\<Omega>. (ubDom\<cdot>sb = In)\<leadsto>if sbHdElemWell sb then ufRestrict In Out\<cdot>(h (Abs_sbElem (inv convDiscrUp (sbHdElem\<cdot>sb)))) \<rightleftharpoons> sb else ubclLeast Out) \<rightleftharpoons> sb = the None" 
+      sorry
+    then show ?thesis
+      apply(simp add: ufLeast_def)
+      by (simp add: False ubclDom_ubundle_def)
+  qed
+qed
+  
+    
 lemma [simp]:"inj_on (\<lambda> h. Abs_ufun (\<Lambda>  sb.  (ubDom\<cdot>sb = In) 
                                               \<leadsto> (if (sbHdElemWell sb) then ufRestrict In Out\<cdot>(h (Abs_sbElem(inv convDiscrUp (sbHdElem\<cdot>sb)))) \<rightleftharpoons> (sbRt\<cdot>sb) else ubclLeast Out))) {h. \<forall>m. ufDom\<cdot>(h m) = In \<and> ufRan\<cdot>(h m) = Out}" (*h must map to spf with dom = In and Range = Out and not map to ufLeast In Out*)
 proof(rule inj_onI)
@@ -247,7 +460,7 @@ lemma spfStep_inj:"inj (Rep_cfun(spfStep In Out))"
   sorry
 
 lemma spfstep_insert: "spfStep In Out\<cdot>h= Abs_ufun (\<Lambda>  sb.  (ubDom\<cdot>sb = In) 
-                                              \<leadsto> (if (sbHdElemWell sb) then ufRestrict In Out\<cdot>(h (Abs_sbElem(inv convDiscrUp (sbHdElem\<cdot>sb)))) \<rightleftharpoons> (sbRt\<cdot>sb) else ubclLeast Out))"
+                                              \<leadsto> (if (sbHdElemWell sb) then ufRestrict In Out\<cdot>(h (Abs_sbElem(inv convDiscrUp (sbHdElem\<cdot>sb)))) \<rightleftharpoons> sb else ubclLeast Out))"
   by(simp add: spfStep_def spfStep_cont)
 
 lemma spfstep_dom[simp]:"ufDom\<cdot>(spfStep cIn cOut\<cdot>f) = cIn"
